messageInvariantPrototypes/toyLeaderElection/decentralizedMonotonic_globalHistory/messageInvariants.dfy
@@ -18,7 +18,7 @@ ghost predicate ValidMessages(c: Constants, v: Variables)
 }
 
 // Send invariant
-ghost predicate VoteReqSendValidity(c: Constants, v: Variables)
+ghost predicate SendVoteReqValidity(c: Constants, v: Variables)
   requires v.WF(c)
   requires ValidMessages(c, v)
 {
@@ -28,12 +28,12 @@ ghost predicate VoteReqSendValidity(c: Constants, v: Variables)
   :: 
   (exists i ::
       && v.ValidHistoryIdxStrict(i)
-      && Host.VoteReqSendFunc(c.hosts[msg.candidate], v.History(i).hosts[msg.candidate], v.History(i+1).hosts[msg.candidate], msg)
+      && Host.SendVoteReq(c.hosts[msg.candidate], v.History(i).hosts[msg.candidate], v.History(i+1).hosts[msg.candidate], msg)
   )
 }
 
 // Send invariant
-ghost predicate VoteSendValidity(c: Constants, v: Variables)
+ghost predicate SendVoteValidity(c: Constants, v: Variables)
   requires v.WF(c)
   requires ValidMessages(c, v)
 {
@@ -43,7 +43,7 @@ ghost predicate VoteSendValidity(c: Constants, v: Variables)
   :: 
   (exists i ::
       && v.ValidHistoryIdxStrict(i)
-      && Host.VoteSendFunc(c.hosts[msg.voter], v.History(i).hosts[msg.voter], v.History(i+1).hosts[msg.voter], msg)
+      && Host.SendVote(c.hosts[msg.voter], v.History(i).hosts[msg.voter], v.History(i+1).hosts[msg.voter], msg)
   )
 }
 
@@ -52,8 +52,8 @@ ghost predicate MessageInv(c: Constants, v: Variables)
   && v.WF(c)
   && ValidHistory(c, v)
   && ValidMessages(c, v)
-  && VoteReqSendValidity(c, v)
-  && VoteSendValidity(c, v)
+  && SendVoteReqValidity(c, v)
+  && SendVoteValidity(c, v)
 }
 
 lemma InitImpliesMessageInv(c: Constants, v: Variables)
@@ -70,17 +70,17 @@ lemma MessageInvInductive(c: Constants, v: Variables, v': Variables)
 {
   assert ValidMessages(c, v');
   InvNextValidHistory(c, v, v');
-  InvNextVoteReqSendValidity(c, v, v');
-  InvNextVoteSendValidity(c, v, v');
+  InvNextSendVoteReqValidity(c, v, v');
+  InvNextSendVoteValidity(c, v, v');
 }
 
-lemma InvNextVoteReqSendValidity(c: Constants, v: Variables, v': Variables)
+lemma InvNextSendVoteReqValidity(c: Constants, v: Variables, v': Variables)
   requires v.WF(c) && v'.WF(c)
   requires ValidHistory(c, v) && ValidHistory(c, v')
   requires ValidMessages(c, v)
-  requires VoteReqSendValidity(c, v)
+  requires SendVoteReqValidity(c, v)
   requires Next(c, v, v')
-  ensures VoteReqSendValidity(c, v')
+  ensures SendVoteReqValidity(c, v')
 {
   forall msg | 
     && msg in v'.network.sentMsgs
@@ -88,23 +88,23 @@ lemma InvNextVoteReqSendValidity(c: Constants, v: Variables, v': Variables)
   ensures
   (exists i ::
       && v'.ValidHistoryIdxStrict(i)
-      && Host.VoteReqSendFunc(c.hosts[msg.candidate], v'.History(i).hosts[msg.candidate], v'.History(i+1).hosts[msg.candidate], msg)
+      && Host.SendVoteReq(c.hosts[msg.candidate], v'.History(i).hosts[msg.candidate], v'.History(i+1).hosts[msg.candidate], msg)
   ) {
     if msg !in v.network.sentMsgs {
       // witness and trigger
       var i := |v.history|-1;
-      assert Host.VoteReqSendFunc(c.hosts[msg.candidate], v'.History(i).hosts[msg.candidate], v'.History(i+1).hosts[msg.candidate], msg);
+      assert Host.SendVoteReq(c.hosts[msg.candidate], v'.History(i).hosts[msg.candidate], v'.History(i+1).hosts[msg.candidate], msg);
     }
   }
 }
 
-lemma InvNextVoteSendValidity(c: Constants, v: Variables, v': Variables)
+lemma InvNextSendVoteValidity(c: Constants, v: Variables, v': Variables)
   requires v.WF(c) && v'.WF(c)
   requires ValidHistory(c, v) && ValidHistory(c, v')
   requires ValidMessages(c, v)
-  requires VoteSendValidity(c, v)
+  requires SendVoteValidity(c, v)
   requires Next(c, v, v')
-  ensures VoteSendValidity(c, v')
+  ensures SendVoteValidity(c, v')
 {
   forall msg | 
     && msg in v'.network.sentMsgs
@@ -112,12 +112,12 @@ lemma InvNextVoteSendValidity(c: Constants, v: Variables, v': Variables)
   ensures
   (exists i ::
       && v'.ValidHistoryIdxStrict(i)
-      && Host.VoteSendFunc(c.hosts[msg.voter], v'.History(i).hosts[msg.voter], v'.History(i+1).hosts[msg.voter], msg)
+      && Host.SendVote(c.hosts[msg.voter], v'.History(i).hosts[msg.voter], v'.History(i+1).hosts[msg.voter], msg)
   ) {
     if msg !in v.network.sentMsgs {
       // witness and trigger
       var i := |v.history|-1;
-      assert Host.VoteSendFunc(c.hosts[msg.voter], v'.History(i).hosts[msg.voter], v'.History(i+1).hosts[msg.voter], msg);
+      assert Host.SendVote(c.hosts[msg.voter], v'.History(i).hosts[msg.voter], v'.History(i+1).hosts[msg.voter], msg);
     }
   }
 }
